DependentComputability/Tactic/Util.lean
@@ -1,0 +1,237 @@
+import Qq
+
+open Lean Meta Qq
+
+def Qq.matchForallQ (e : Expr) : MetaM (Option ((u v : Level) × (α : Q(Sort u)) × Q($α → Sort v))) := do
+  let .forallE nm t b bi := id e | return none
+  let u ← getLevel t
+  have t : Q(Sort u) := t
+  withLocalDeclQ nm bi q($t) fun x => do
+    let v ← getLevel (b.instantiate1 x)
+    return some ⟨u, v, q($t), .lam nm t b bi⟩
+
+def Qq.matchLambdaQ (e : Expr) : MetaM (Option ((u v : Level) × (α : Q(Sort u)) × (β : Q($α → Sort v)) × Q((a : $α) → $β a))) := do
+  let .lam nm t b bi := e | return none
+  let u ← getLevel t
+  have t : Q(Sort u) := t
+  withLocalDeclQ nm bi q($t) fun x => do
+    let bty ← inferType (b.instantiate1 x)
+    let v ← getLevel bty
+    return some ⟨u, v, q($t), .lam nm t (bty.abstract #[x]) bi, e⟩
+
+@[inline]
+def Qq.isAlwaysZeroQ (lvl : Level) : MaybeLevelDefEq lvl Level.zero :=
+  if lvl.isAlwaysZero then
+    .defEq ⟨⟩
+  else
+    .notDefEq
+
+@[inline]
+def Qq.withLetDeclQ [MonadControlT MetaM n] [Monad n]
+    (name : Name) {type : Q(Sort u)} (val : Q($type))
+    (k : (var : Q($type)) → $var =Q $val → n α) : n α :=
+  withLetDecl name type val (fun e => k e ⟨⟩)
+
+@[inline]
+def Qq.withHaveDeclQ [MonadControlT MetaM n] [Monad n]
+    (name : Name) {type : Q(Sort u)} (val : Q($type))
+    (k : (var : Q($type)) → n α) : n α :=
+  withLetDecl name type val k (nondep := true)
+
+/-- Returns whether the recursor has large elimination, i.e. whether it can eliminate into any universe. -/
+def Lean.RecursorVal.largeElim (val : RecursorVal) : Bool :=
+  go val.numParams val.type
+where
+  go : Nat → Expr → Bool
+    | 0, .forallE _ t _ _ => (t.getForallBody matches .sort (.param _))
+    | k + 1, .forallE _ _ b _ => go k b
+    | _, _ => false
+
+set_option doc.verso true in
+/--
+Returns a list of all recursors mutual with this one.
+See also {name}`RecursorVal.all` which produces a list of inductives.
+-/
+def Lean.RecursorVal.allRecs (val : RecursorVal) : List Name := Id.run do
+  let fst :: more := val.all | return []
+  let numNested := val.numMotives - val.all.length
+  let fstRec := mkRecName fst
+  return fstRec :: (more.map mkRecName ++ (List.range' 1 numNested).map fstRec.appendIndexAfter)
+
+local syntax (name := matchQqConstApp) "match_qq_const_app" term:arg term:arg term:arg* ";" term:arg term:arg : term
+local syntax (name := doMatchQqConstApp) "match_qq_const_app" term:arg term:arg term:arg* ";" doSeq doSeq : doElem
+
+set_option backward.do.legacy false
+open Elab Term
+elab_rules : term <= exp
+  | `(match_qq_const_app $x:term $fn:term $args:term*; $alt:term $default:term) => do
+    let (ident, explicit, levels) ← match fn with
+      | `($id:ident) => pure (id, false, #[])
+      | `(@$id:ident) => pure (id, true, #[])
+      | `($id:ident.{$us,*}) => pure (id, false, us.getElems)
+      | `(@$id:ident.{$us,*}) => pure (id, true, us.getElems)
+      | _ => throwErrorAt fn "Invalid raw Qq match, expected identifier"
+    let levels ← levels.mapM fun lvl => match lvl with
+      | `($id:ident) => pure id
+      | `(_) => withFreshMacroScope `(u)
+      | _ => throwErrorAt lvl "Invalid pattern, expected identifier"
+    let args ← args.mapM fun arg => match arg with
+      | `($id:ident) => pure id
+      | `(_) => withFreshMacroScope `(x)
+      | _ => throwErrorAt arg "Invalid pattern, expected identifier"
+    let nm ← realizeGlobalConstNoOverloadWithInfo ident
+    let info ← withRef fn <| getConstVal nm
+    if levels.size > info.levelParams.length then
+      throwErrorAt (mkNullNode (levels.drop info.levelParams.length)) "Too many level parameters"
+    let mut levels := levels
+    while levels.size < info.levelParams.length do
+      levels := levels.push (← withFreshMacroScope `(ident| u))
+    let quotedType ← forallBoundedTelescope info.type args.size fun vars body => do
+      if args.size > vars.size then
+        throwErrorAt (mkNullNode (args.drop vars.size)) "Too many arguments"
+      let levelVarInfos := levels.map (fun x => (x.getId, q(Level)))
+      withLocalDeclsDND levelVarInfos fun levelVars => do
+      let rec go (i : Nat) (qqVars : Array Expr) : Impl.QuoteM Expr := do
+        if h : i < vars.size then
+          let decl ← vars[i].fvarId!.getDecl
+          let qqVarType : Q(Expr) ← Impl.quoteExpr decl.type
+          let qqVarType := q(Quoted $qqVarType)
+          withLocalDeclD args[i]!.getId qqVarType fun qqVar => do
+            withReader (fun state => { state with exprBackSubst := state.exprBackSubst.insert decl.toExpr (.quoted qqVar) }) do
+              go (i + 1) (qqVars.push qqVar)
+        else
+          let qqResType : Q(Expr) ← Impl.quoteExpr body
+          let qqResLevel : Q(Level) ← Impl.quoteLevel (← getLevel body)
+          let qqApp : Q(Expr) ← Impl.quoteExpr (mkAppN (.const nm (info.levelParams.map Level.param)) vars)
+          mkLambdaFVars qqVars q(($qqResType, $qqResLevel, $qqApp))
+      let mut levelBackSubst : Std.HashMap Level Expr := {}
+      for param in info.levelParams, var in levelVars do
+        levelBackSubst := levelBackSubst.insert (.param param) var
+      let ctx := {
+        mayPostpone := false
+        levelNames := levels.map (·.getId) |>.toList
+        levelBackSubst
+      }
+      (go 0 levelVars).run ctx
+    let discr ← elabTermEnsuringTypeQ x q(Expr)
+    let (altBranch, altType) ← lambdaTelescope quotedType fun qqVars qqBody => do
+      for lvl in levels, qqVar in qqVars do
+        addTermInfo' (isBinder := true) lvl qqVar
+      for arg in args, qqVar in qqVars[levels.size...*] do
+        addTermInfo' (isBinder := true) arg qqVar
+      if let `($id:ident) := x then
+        let_expr Prod.mk _ _ resType more := qqBody | unreachable!
+        let_expr Prod.mk _ _ resLvl resVal := more | unreachable!
+        have resLvl : Q(Level) := resLvl
+        have resType : Q(Quoted (.sort $resLvl)) := resType
+        have resVal : Q(Quoted $resType) := resVal
+        withHaveDeclQ id.getId (type := q(Quoted $resType)) discr fun var => do
+        let eqName ← mkFreshUserName (id.getId.appendAfter "_eq")
+        have discr : Q(Quoted $resType) := var
+        withHaveDeclQ eqName (type := q(@QuotedDefEq $resLvl (Quoted.unsafeMk $resType) (Quoted.unsafeMk $discr) (Quoted.unsafeMk $resVal))) q(.unsafeIntro) fun eqVar => do
+          let res ← elabTermEnsuringType alt exp
+          let qqVars' := qqVars.push var |>.push eqVar
+          return (← mkLetFVars qqVars' res (generalizeNondepLet := false), ← mkForallFVars qqVars exp)
+      else
+        let res ← elabTermEnsuringType alt exp
+        return (← mkLambdaFVars qqVars res, ← mkForallFVars qqVars exp)
+    let expLevel ← getLevel exp
+    have exp : Q(Sort expLevel) := exp
+    let defaultBranch : Q($exp) ← elabTermEnsuringType default exp
+    let defaultBranch := q(fun _ : Unit => $defaultBranch)
+    withLetDecl `alt altType altBranch (nondep := true) fun altBranch => do
+    withLetDecl `default q(Unit → $exp) defaultBranch (nondep := true) fun (defaultBranch : Q(Unit → $exp)) => do
+      let rec goLevels (discr : Q(List Level)) (revArgs : Array Q(Expr)) (levelVars : Array Q(Level)) (i : Nat) : MetaM Q($exp) := do
+        if h : i < levels.size then
+          let further : Q(Level → List Level → $exp) ← withLocalDeclD `u q(Level) fun uvar => do
+            withLocalDeclD `us q(List Level) fun usvar => do
+              let res ← goLevels usvar revArgs (levelVars.push uvar) (i + 1)
+              mkLambdaFVars #[uvar, usvar] res
+          return q(($discr).casesOn ($defaultBranch ()) $further)
+        else
+          have res : Q($exp) := mkAppRev (mkAppN altBranch levelVars) revArgs
+          return q(($discr).casesOn $res (fun _ _ => $defaultBranch ()))
+      termination_by levels.size - i
+      let rec goMatch (discr : Q(Expr)) (revArgs : Array Q(Expr)) (n : Nat) : MetaM Q($exp) := do
+        match n with
+        | 0 =>
+          let further : Q(List Level → $exp) ← withLocalDeclD `lvls q(List Level) fun lvlsVar => do
+            let res ← goLevels lvlsVar revArgs #[] 0
+            mkLambdaFVars #[lvlsVar] res
+          have nm : Name := nm
+          return q(
+            if h : ($discr).isConstOf $nm then
+              have lvls := ($discr).constLevels!
+              $further lvls
+            else $defaultBranch ())
+        | n + 1 =>
+          let further : Q(Expr → Expr → $exp) ← withLocalDeclD `fn q(Expr) fun fnVar => do
+            withLocalDeclD `arg q(Expr) fun argVar => do
+              let res ← goMatch fnVar (revArgs.push argVar) n
+              mkLambdaFVars #[fnVar, argVar] res
+          return q(
+            if h : ($discr).isApp then
+              have fn := ($discr).appFn h
+              have arg := ($discr).appArg h
+              $further fn arg
+            else $defaultBranch ())
+      let res ← goMatch discr #[] args.size
+      mkLetFVars #[altBranch, defaultBranch] res (generalizeNondepLet := false)
+
+macro_rules
+  | `(match $x:term with | q($fn $args*) => $alt:term | _ => $default:term) => do
+    let args ← args.mapM fun stx => do
+      let stx := stx.raw
+      if stx.isAntiquot && !stx.isEscapedAntiquot then
+        return ⟨stx.getAntiquotTerm⟩
+      else
+        Macro.throwUnsupported
+    `(match_qq_const_app $x:term $fn:term $args:term*; $alt:term $default:term)
+
+open Elab Parser Term Do in
+@[doElem_elab doMatchQqConstApp]
+def elabDoMatchQqConstApp : DoElab := fun stx dec => do
+  let `(doElem| match_qq_const_app $x:term $fn:term $args:term*; $alt:doSeq $default:doSeq) := stx |
+    throwUnsupportedSyntax
+  let doBlockResultType := (← read).doBlockResultType
+  let mγ ← mkMonadicType doBlockResultType
+  let info ← inferControlInfoElem stx
+  dec.withDuplicableCont info fun dec => do
+  let mut argsIdents ← args.filterMapM fun arg => match arg with
+    | `($id:ident) => pure (some id)
+    | `(_) => pure none
+    | _ => throwErrorAt arg "Invalid pattern, expected identifier"
+  if let `($id:ident) := x then
+    argsIdents := argsIdents.push id
+  checkMutVarsForShadowing argsIdents
+  doElabToSyntax m!"match_qq_const_app alternative" (ref := alt) (elabDoSeq alt dec) fun alt => do
+  doElabToSyntax m!"match_qq_const_app alternative" (ref := default) (elabDoSeq default dec) fun default => do
+    Term.elabTerm (← `(match_qq_const_app $x:term $fn:term $args:term*; $alt:term $default:term)) mγ
+
+open Elab Do in
+@[doElem_control_info doMatchQqConstApp]
+def doMatchQqConstAppControlInfo : ControlInfoHandler := fun stx => do
+  let `(doElem| match_qq_const_app $_:term $_:term $_:term*; $alt:doSeq $default:doSeq) := stx |
+    throwUnsupportedSyntax
+  return (← inferControlInfoSeq alt).alternative (← inferControlInfoSeq default)
+
+macro_rules
+  | `(doElem| match $x:term with | q($fn $args*) => $alt:doSeq | _ => $default:doSeq) => do
+    let args ← args.mapM fun stx => do
+      let stx := stx.raw
+      if stx.isAntiquot && !stx.isEscapedAntiquot then
+        return ⟨stx.getAntiquotTerm⟩
+      else
+        Macro.throwUnsupported
+    `(doElem| match_qq_const_app $x:term $fn:term $args:term*; $alt:doSeq $default:doSeq)
+
+macro_rules
+  | `(doElem| let q($fn $args*) := $x:term | $otherwise $(body?)?) => do
+    let body ← body?.getDM `(Parser.Term.doSeqIndent| pure PUnit.unit)
+    let args ← args.mapM fun stx => do
+      let stx := stx.raw
+      if stx.isAntiquot && !stx.isEscapedAntiquot then
+        return ⟨stx.getAntiquotTerm⟩
+      else
+        Macro.throwUnsupported
+    `(doElem| match_qq_const_app $x:term $fn:term $args:term*; $body:doSeqIndent $otherwise:doSeqIndent)
